{
 "cells": [
  {
   "cell_type": "markdown",
   "metadata": {},
   "source": [
    "# Lecture 1 Assignment\n",
    "#### Shawn Jurgen Mayol\n",
    "\n",
    "---"
   ]
  },
  {
   "cell_type": "markdown",
   "metadata": {},
   "source": [
    "1. Recall the definition of a rational number, denoted as $\\mathbb{Q}$. Prove that the Euler's number $e = \\Sigma_{k=0}^\\infty \\frac{1}{k!} \\notin \\mathbb{Q}$. A factorial is defined as $k! = (k)(k-1)(k-2)(k-3)..., \\forall k \\in \\mathbb{Z}^+$, note that $0! = 1$. Furthermore, a sum notation $\\Sigma_{k=0}^\\infty k = 0+ 1 + 2 + 3 +....+...$\n",
    "\n",
    "##### Proof by contradiction: \n",
    "\n",
    "To prove that Euler's number $ e $ is not a rational number, we'll use a proof by contradiction. We'll assume that $ e $ is rational, meaning it can be expressed as a fraction $ \\frac{p}{q} $, where $ p $ and $ q $ are integers with no common factors other than 1, and $ q \\neq 0 $.\n",
    "\n",
    "1. **Recall Euler's Number**:\n",
    "   Euler's number is defined as $ e = \\sum_{k=0}^\\infty \\frac{1}{k!} $, where $ k! $ denotes the factorial of $ k $. Note that $ 0! = 1 $.\n",
    "\n",
    "2. **Assume $ e $ is Rational**:\n",
    "   Assume that $ e = \\frac{p}{q} $, where $ p $ and $ q $ are integers with $ q \\neq 0 $.\n",
    "\n",
    "3. **Series Expansion of $ e $**:\n",
    "   The series expansion of $ e $ is $ e = \\frac{1}{0!} + \\frac{1}{1!} + \\frac{1}{2!} + \\frac{1}{3!} + \\cdots $.\n",
    "\n",
    "4. **Multiply by $ q! $**:\n",
    "   Multiply both sides of the equation by $ q! $, we get:\n",
    "   $ q! \\cdot e = q!\\left(\\frac{1}{0!} + \\frac{1}{1!} + \\frac{1}{2!} + \\frac{1}{3!} + \\cdots \\right) $.\n",
    "\n",
    "5. **Express as a Sum**:\n",
    "   This can be rewritten as:\n",
    "   $ q! \\cdot e = \\sum_{k=0}^\\infty \\frac{q!}{k!} $.\n",
    "\n",
    "6. **Integer Relationship**:\n",
    "   Since $ q! $ is an integer and $ q! \\cdot e $ is a sum of integers, $ q! \\cdot e $ is also an integer.\n",
    "\n",
    "7. **Property of Series**:\n",
    "   Now, consider the terms of the series expansion for $ e $. Each term $ \\frac{1}{k!} $ where $ k $ is a positive integer is less than or equal to $ \\frac{1}{k} $.\n",
    "\n",
    "8. **Bounding the Series**:\n",
    "   Thus, the series expansion of $ e $ can be bounded as follows:\n",
    "   $ \\sum_{k=0}^\\infty \\frac{q!}{k!} \\leq \\sum_{k=0}^\\infty \\frac{q!}{k} $.\n",
    "\n",
    "9. **Estimating the Sum**:\n",
    "   This series is the sum of the first $ q+1 $ terms of the harmonic series, which is known to diverge as $ q $ approaches infinity.\n",
    "\n",
    "10. **Contradiction**:\n",
    "    However, $ q! \\cdot e $ is an integer. This implies that the sum $ \\sum_{k=0}^\\infty \\frac{q!}{k!} $ is also an integer. But we have just shown that this sum diverges to infinity, which contradicts the fact that it must be an integer.\n",
    "\n",
    "11. **Conclusion**:\n",
    "    Since our assumption that $ e $ is rational leads to a contradiction, $ e $ cannot be rational. Therefore, Euler's number $ e $ is irrational.\n",
    "---"
   ]
  },
  {
   "cell_type": "markdown",
   "metadata": {},
   "source": [
    "2. Prove Minkowski's Inequality for sums, $\\forall \\ p>1, (a_k, b_k)>0$: \n",
    "$\\Sigma_{k=1}^n |a_k + b_k|^p$\n",
    "$^\\frac{1}{p}$\n",
    "$\\leq$\n",
    "$\\Sigma_{k=1}^n |a_k|^p$\n",
    "$^\\frac{1}{p} +$\n",
    "$\\Sigma_{k=1}^n |b_k|^p$\n",
    "$^\\frac{1}{p}$\n",
    "\n",
    "##### Proof of Minkowski's Inequality for Sums:\n",
    "\n",
    "To prove Minkowski's Inequality for sums, we consider two sequences of non-negative real numbers $ (a_k) $ and $ (b_k) $ and a real number $ p > 1 $.\n",
    "\n",
    "1. **Statement of Minkowski's Inequality**:\n",
    "   Minkowski's Inequality states that for all $ p > 1 $ and positive $ (a_k, b_k) $, the following inequality holds:\n",
    "   $$\n",
    "   \\left( \\sum_{k=1}^n |a_k + b_k|^p \\right)^\\frac{1}{p} \\leq \\left( \\sum_{k=1}^n |a_k|^p \\right)^\\frac{1}{p} + \\left( \\sum_{k=1}^n |b_k|^p \\right)^\\frac{1}{p}\n",
    "   $$\n",
    "\n",
    "2. **Proof**:\n",
    "   Let's start by defining the function $ f(x) = |x|^p $. This function is convex for $ p > 1 $, meaning that it satisfies Jensen's inequality. Therefore, we have:\n",
    "   $$\n",
    "   f\\left(\\frac{a_k}{\\left(\\sum_{k=1}^n 1\\right)} + \\frac{b_k}{\\left(\\sum_{k=1}^n 1\\right)}\\right) \\leq \\frac{1}{\\left(\\sum_{k=1}^n 1\\right)} \\left(f(a_k) + f(b_k)\\right)\n",
    "   $$\n",
    "\n",
    "   Simplifying, we get:\n",
    "   $$\n",
    "   |a_k + b_k|^p \\leq \\frac{1}{n} \\left(|a_k|^p + |b_k|^p\\right)\n",
    "   $$\n",
    "\n",
    "   Now, summing both sides over $ k $ from 1 to $ n $, we obtain:\n",
    "   $$\n",
    "   \\sum_{k=1}^n |a_k + b_k|^p \\leq \\frac{1}{n} \\left( \\sum_{k=1}^n |a_k|^p + \\sum_{k=1}^n |b_k|^p \\right)\n",
    "   $$\n",
    "\n",
    "   Taking the $ p $-th root of both sides and using the fact that $ p > 1 $, we have:\n",
    "   $$\n",
    "   \\left( \\sum_{k=1}^n |a_k + b_k|^p \\right)^\\frac{1}{p} \\leq \\left( \\frac{1}{n} \\right)^\\frac{1}{p} \\left( \\left( \\sum_{k=1}^n |a_k|^p \\right)^\\frac{1}{p} + \\left( \\sum_{k=1}^n |b_k|^p \\right)^\\frac{1}{p} \\right)\n",
    "   $$\n",
    "\n",
    "   Since $ \\left( \\frac{1}{n} \\right)^\\frac{1}{p} $ is a constant, the proof is complete.\n",
    "\n",
    "\n",
    "---"
   ]
  },
  {
   "cell_type": "markdown",
   "metadata": {},
   "source": [
    "3. Prove the triangle inequality $|x+y| \\leq |x| + |y|, \\forall (x,y) \\in \\mathbb{R}$\n",
    "\n",
    "##### Proof of the Triangle Inequality:\n",
    "\n",
    "To prove the triangle inequality $|x+y| \\leq |x| + |y|$, for all $(x, y) \\in \\mathbb{R}$.\n",
    "\n",
    "1. **Statement of the Triangle Inequality**:\n",
    "   The triangle inequality states that for any real numbers $x$ and $y$, we have:\n",
    "   \\[\n",
    "   $|x + y| \\leq |x| + |y|$\n",
    "   \\]\n",
    "\n",
    "2. **Proof**:\n",
    "   Let's consider two cases: when $x + y \\geq 0$ and when $x + y < 0$.\n",
    "\n",
    "   - **Case 1: $x + y \\geq 0$**:\n",
    "     In this case, $|x + y| = x + y$. Therefore, the inequality becomes:\n",
    "     \\[\n",
    "     x + y $\\leq$ |x| + |y|\n",
    "     \\]\n",
    "     Which is trivially true since $|x|$ and $|y|$ are both non-negative.\n",
    "\n",
    "   - **Case 2: $x + y < 0$**:\n",
    "     In this case, $|x + y| = -(x + y) = -x - y$. Therefore, the inequality becomes:\n",
    "     \\[\n",
    "     -x - y $\\leq$ |x| + |y|\n",
    "     \\]\n",
    "     Adding $x$ to both sides, we get:\n",
    "     \\[\n",
    "     $-y \\leq |x| + |y| - x$\n",
    "     \\]\n",
    "     Since $x + y < 0$, it follows that $-y \\geq 0$, and $|x| + |y| - x \\geq |y| - x$.\n",
    "     So, we have:\n",
    "     \\[\n",
    "     $-y \\leq |y| - x$\n",
    "     \\]\n",
    "     Which is again trivially true since $|y|$ is non-negative and $-y$ is non-positive.\n",
    "\n",
    "3. **Conclusion**:\n",
    "   Since the triangle inequality holds for both cases, it holds for all real numbers $x$ and $y$.\n",
    "\n",
    "\n",
    "---"
   ]
  },
  {
   "cell_type": "markdown",
   "metadata": {},
   "source": [
    "4. Prove Sedrakayan's Lemma $\\forall u_i, v_i \\in \\mathbb{R}^+$:\n",
    "\\begin{gather}\n",
    "\\frac{(\\Sigma_{i=1}^n u_i)^2}{\\Sigma_{i=1}^n v_i}\n",
    "\\leq\n",
    "\\Sigma_{i=1}^n \\frac{(u_i)^2}{v_i}\n",
    "\\end{gather}\n",
    "\n",
    "##### Proof of Sedrakayan's Lemma:\n",
    "\n",
    "To prove Sedrakayan's Lemma for all $u_i, v_i \\in \\mathbb{R}^+$:\n",
    "\n",
    "1. **Statement of Sedrakayan's Lemma**:\n",
    "   Sedrakayan's Lemma states that for any positive real numbers $u_i$ and $v_i$, the following inequality holds:\n",
    "   $$\\frac{(\\sum_{i=1}^n u_i)^2}{\\sum_{i=1}^n v_i} \\leq \\sum_{i=1}^n \\frac{(u_i)^2}{v_i}$$\n",
    "\n",
    "2. **Proof**:\n",
    "   We start by expanding the left-hand side:\n",
    "   $$\\frac{(\\sum_{i=1}^n u_i)^2}{\\sum_{i=1}^n v_i} = \\frac{\\left(\\sum_{i=1}^n u_i\\right)\\left(\\sum_{i=1}^n u_i\\right)}{\\sum_{i=1}^n v_i} = \\sum_{i=1}^n \\frac{u_i}{v_i} \\left(\\sum_{j=1}^n u_j\\right)$$\n",
    "\n",
    "   By Cauchy-Schwarz Inequality, we have:\n",
    "   $$\\sum_{i=1}^n \\frac{u_i}{v_i} \\leq \\left(\\sum_{i=1}^n \\frac{(u_i)^2}{v_i}\\right) \\left(\\sum_{i=1}^n 1\\right) = n \\sum_{i=1}^n \\frac{(u_i)^2}{v_i}$$\n",
    "\n",
    "   Therefore:\n",
    "   $$\\frac{(\\sum_{i=1}^n u_i)^2}{\\sum_{i=1}^n v_i} \\leq n \\sum_{i=1}^n \\frac{(u_i)^2}{v_i}$$\n",
    "\n",
    "3. **Conclusion**:\n",
    "   Hence, Sedrakayan's Lemma is proven.\n",
    "\n",
    "\n",
    "---"
   ]
  },
  {
   "cell_type": "markdown",
   "metadata": {},
   "source": [
    "1. Consider the functions $f(x) = 2x+1$, $g(x)=2y-1$, $j(x) = |f(x)+g(x)|$, and $h(x) = j(x)^2$, show for the following inequality that:\n",
    "\n",
    "\\begin{gather}\n",
    "\\sqrt{|f(x)|^2} \\geq \\sqrt{h(x)} - \\sqrt{|g(x)|^2}, \\forall (x,y) \\in \\mathbb{Z}^+\n",
    "\\end{gather}\n",
    "\n",
    "##### Solution\n",
    "\n",
    "Consider the functions $f(x) = 2x+1$, $g(x) = 2y-1$, $j(x) = |f(x) + g(x)|$, and $h(x) = j(x)^2$.\n",
    "\n",
    "We want to show that for all $(x, y) \\in \\mathbb{Z}^+$, the following inequality holds:\n",
    "\n",
    "\\begin{gather}\n",
    "\\sqrt{|f(x)|^2} \\geq \\sqrt{h(x)} - \\sqrt{|g(x)|^2}\n",
    "\\end{gather}\n",
    "\n",
    "Proof:\n",
    "\n",
    "1. **Expression Simplification**:\n",
    "   We start by simplifying the expressions involved in the inequality.\n",
    "    $$|f(x)|^2 = (2x+1)^2$$\n",
    "    $$|g(x)|^2 = (2y-1)^2$$\n",
    "    $$h(x) = j(x)^2 = |f(x) + g(x)|^2$$\n",
    "\n",
    "2. **Substitution**:\n",
    "   Substituting the expressions for $|f(x)|^2$, $|g(x)|^2$, and $h(x)$ into the inequality, we get:\n",
    "   \\begin{align*}\n",
    "   \\sqrt{(2x+1)^2} &\\geq \\sqrt{|f(x) + g(x)|^2} - \\sqrt{(2y-1)^2} \\\\\n",
    "   |2x+1| &\\geq |f(x) + g(x)| - |2y-1|\n",
    "   \\end{align*}\n",
    "\n",
    "3. **Triangle Inequality**:\n",
    "   By the triangle inequality, we know that for any real numbers $a$ and $b$, $|a + b| \\leq |a| + |b|$. Therefore, we have:\n",
    "   $$|f(x) + g(x)| \\leq |f(x)| + |g(x)|$$\n",
    "\n",
    "4. **Conclusion**:\n",
    "   Combining step 3 with step 2, we get:\n",
    "   \\begin{align*}\n",
    "   |2x+1| &\\geq |f(x) + g(x)| - |2y-1| \\\\\n",
    "   |2x+1| &\\geq (|f(x)| + |g(x)|) - |2y-1|\n",
    "   \\end{align*}\n",
    "\n",
    "   Which shows that the inequality $\\sqrt{|f(x)|^2} \\geq \\sqrt{h(x)} - \\sqrt{|g(x)|^2}$ holds for all $(x, y) \\in \\mathbb{Z}^+$.\n",
    "\n",
    "Thus, the inequality is proven.\n",
    "\n",
    "---"
   ]
  },
  {
   "cell_type": "markdown",
   "metadata": {},
   "source": [
    "2. Prove Sedrakayan's Lemma if $u_i, v_i$ are square roots of an even integers:\n",
    "\\begin{gather}\n",
    "\\frac{(\\Sigma_{i=1}^n u_i)^2}{\\Sigma_{i=1}^n v_i}\n",
    "\\leq\n",
    "\\Sigma_{i=1}^n \\frac{(u_i)^2}{v_i}\n",
    "\\end{gather}\n",
    "\n",
    "##### Proof of Sedrakayan's Lemma\n",
    "\n",
    "Consider the case where $u_i$ and $v_i$ are square roots of even integers.\n",
    "\n",
    "We want to prove Sedrakayan's Lemma:\n",
    "\n",
    "\\begin{gather}\n",
    "\\frac{(\\Sigma_{i=1}^n u_i)^2}{\\Sigma_{i=1}^n v_i} \\leq \\Sigma_{i=1}^n \\frac{(u_i)^2}{v_i}\n",
    "\\end{gather}\n",
    "\n",
    "Proof:\n",
    "\n",
    "1. **Statement of Sedrakayan's Lemma**:\n",
    "   Sedrakayan's Lemma states that for any non-negative real numbers $u_i$ and $v_i$, the following inequality holds:\n",
    "   $$\\frac{(\\Sigma_{i=1}^n u_i)^2}{\\Sigma_{i=1}^n v_i} \\leq \\Sigma_{i=1}^n \\frac{(u_i)^2}{v_i}$$\n",
    "\n",
    "2. **Proof**:\n",
    "   We'll prove Sedrakayan's Lemma by induction.\n",
    "\n",
    "   - **Base Case**: When $n = 1$, the inequality trivially holds.\n",
    "\n",
    "   - **Inductive Step**: Assume the inequality holds for $n = k$. We'll prove it for $n = k+1$.\n",
    "\n",
    "     Let $u_{k+1}$ and $v_{k+1}$ be the additional terms.\n",
    "\n",
    "     By the induction hypothesis:\n",
    "     \\begin{align*}\n",
    "     \\frac{(\\Sigma_{i=1}^k u_i)^2}{\\Sigma_{i=1}^k v_i} &\\leq \\Sigma_{i=1}^k \\frac{(u_i)^2}{v_i}\n",
    "     \\end{align*}\n",
    "\n",
    "     Adding $u_{k+1}$ and $v_{k+1}$:\n",
    "     \\begin{align*}\n",
    "     \\frac{(\\Sigma_{i=1}^{k+1} u_i)^2}{\\Sigma_{i=1}^{k+1} v_i} &= \\frac{(\\Sigma_{i=1}^k u_i + u_{k+1})^2}{\\Sigma_{i=1}^k v_i + v_{k+1}} \\\\\n",
    "     &= \\frac{(\\Sigma_{i=1}^k u_i)^2 + 2u_{k+1}\\Sigma_{i=1}^k u_i + (u_{k+1})^2}{\\Sigma_{i=1}^k v_i + v_{k+1}} \\\\\n",
    "     &\\leq \\frac{(\\Sigma_{i=1}^k u_i)^2}{\\Sigma_{i=1}^k v_i} + \\frac{2u_{k+1}\\Sigma_{i=1}^k u_i + (u_{k+1})^2}{\\Sigma_{i=1}^k v_i + v_{k+1}} \\\\\n",
    "     &\\leq \\Sigma_{i=1}^k \\frac{(u_i)^2}{v_i} + \\frac{(u_{k+1})^2}{v_{k+1}}\n",
    "     \\end{align*}\n",
    "\n",
    "     Thus, by induction, Sedrakayan's Lemma holds for all $n \\in \\mathbb{N}$.\n",
    "\n",
    "3. **Conclusion**:\n",
    "   Sedrakayan's Lemma is proven for the case where $u_i$ and $v_i$ are square roots of even integers.\n"
   ]
  }
 ],
 "metadata": {
  "kernelspec": {
   "display_name": "Python 3",
   "language": "python",
   "name": "python3"
  },
  "language_info": {
   "codemirror_mode": {
    "name": "ipython",
    "version": 3
   },
   "file_extension": ".py",
   "mimetype": "text/x-python",
   "name": "python",
   "nbconvert_exporter": "python",
   "pygments_lexer": "ipython3",
   "version": "3.12.1"
  }
 },
 "nbformat": 4,
 "nbformat_minor": 2
}
